Remove beq_var and beq_msg; cleanup Env
This commit replaces all remaining uses of beq_var by eq_Var_dec, thus
rendering the former obsolete. It alse removes beq_Sty and beq_msg,
which we never used anyway.

To accomodate this change, a lot of proofs needed to be changed
slightly. The only bigger change is in WfAlt, where we introduce some
limited automation for Ok/Checked inversion in order to make the proofs
significantly simpler.

We also delete large portions of Env.v because they are not currently
used.

src/Subst.v
@@ -1,4 +1,5 @@
 Require Import Sty Var.
+Require Import Coq.Bool.DecBool.
 
 Create HintDb subst discriminated.
 
@@ -9,7 +10,7 @@ Fixpoint subst (x : Var) (r : Sty) (orig : Sty) : Sty :=
   | recv msg tail => recv msg (subst x r tail)
   | ichoice tail1 tail2 => ichoice (subst x r tail1) (subst x r tail2)
   | echoice tail1 tail2 => echoice (subst x r tail1) (subst x r tail2)
-  | mu y tail => if beq_var x y then orig else mu y (subst x r tail)
-  | var y => if beq_var x y then r else orig
+  | mu y tail => ifdec (eq_Var_dec x y) orig (mu y (subst x r tail))
+  | var y => ifdec (eq_Var_dec x y) r orig
   end
 .
