src/Env.v
@@ -1,6 +1,3 @@
-(* TODO This file could probably do with a little more structure, consistent
-   naming and such. *)
-
 Require Import Tac Var.
 Require Import MSetWeakList MSetProperties Program.Basics.
 
@@ -12,64 +9,7 @@ Notation Env := S.t.
 Notation env_empty := S.empty.
 Notation env_add := S.add.
 Notation env_mem := S.In.
-Notation env_memb := SF.In_dec.
-Notation env_eq := S.Equal.
-Notation env_subset := S.Subset.
-Notation env_union := S.union.
-Notation env_singleton x := (env_add x env_empty).
-Notation env_fold := S.fold.
-Notation list_to_env := SF.of_list.
 
-Lemma env_mem_spec_subset :
-  forall x e e',
-  env_subset e e' ->
-  env_mem x e ->
-  env_mem x e'.
-Proof. intros. eapply SF.in_subset; eauto. Qed.
-
-Definition env_subset_equal :
-  forall XS YS,
-  env_eq XS YS ->
-  env_subset XS YS
-  := SF.subset_equal.
-
-Definition env_add_assoc :
-  forall XS X Y,
-  env_eq (env_add X (env_add Y XS)) (env_add Y (env_add X XS))
-  := SF.add_add.
-
-Instance env_add_m_subset (x : Var) : Proper (env_subset ==> env_subset) (env_add x).
-Proof. solve_proper. Qed.
-
-Definition env_union_list (xs : Env) (ys : list Var) : Env :=
-  fold_left (flip env_add) ys xs.
-
-Lemma env_union_list_neutral :
-  forall xs,
-  env_union_list xs nil = xs.
-Proof. auto. Qed.
-
-Lemma env_add_twice :
-  forall X XS,
-  env_eq (env_add X (env_add X XS)) (env_add X XS).
-Proof. intros. apply SF.add_equal. apply S.add_spec; auto. Qed.
-
-Lemma env_add_eq :
-  forall e e' x,
-  env_eq e e' ->
-  env_eq (env_add x e) (env_add x e').
-Proof. intros e e' x eqee'. apply SF.Dec.F.add_m; auto. Qed.
-
-Lemma env_add_mem :
-  forall e x y,
-  env_mem x e ->
-  env_mem x (env_add y e).
-Proof. intros e x y H. apply S.add_spec; auto. Qed.
-
-Lemma env_add_mem' :
-  forall e x,
-  env_mem x (env_add x e).
-Proof. intros. apply SF.Dec.F.add_1. auto. Qed.
 
 Lemma env_mem_add :
   forall e x y,
@@ -78,102 +18,21 @@ Lemma env_mem_add :
   env_mem y e.
 Proof. apply SF.Dec.F.add_3. Qed.
 
-Lemma env_mem_empty : forall x, not (env_mem x env_empty).
+
+Lemma env_add_mem :
+  forall e x y,
+  env_mem x e ->
+  env_mem x (env_add y e).
+Proof. intros e x y H. apply S.add_spec; auto. Qed.
+
+
+Lemma env_add_mem' :
+  forall e x,
+  env_mem x (env_add x e).
+Proof. intros. apply SF.Dec.F.add_1. auto. Qed.
+
+
+Lemma env_mem_empty :
+  forall x,
+  ~ (env_mem x env_empty).
 Proof. unfold not. apply SF.FM.empty_iff. Qed.
-Hint Resolve env_mem_empty : env.
-
-Lemma env_eq_spec :
-  forall e e',
-  env_eq e e' <-> (forall x, env_mem x e <-> env_mem x e').
-Proof. intros; split; intros H; auto. Qed.
-
-Definition env_eq_refl :
-  forall e,
-  env_eq e e
-  := SF.equal_refl.
-
-Definition env_eq_sym :
-  forall e e',
-  env_eq e e' ->
-  env_eq e' e
-  := SF.equal_sym.
-
-Definition env_eq_trans :
-  forall e1 e2 e3,
-  env_eq e1 e2 ->
-  env_eq e2 e3 ->
-  env_eq e1 e3
-  := SF.equal_trans.
-
-Lemma env_add_union_singleton :
-  forall e X,
-  env_eq (env_union e (env_singleton X)) (env_add X e).
-Proof.
-  intros e X. symmetry. rewrite SF.union_sym. apply SF.add_union_singleton.
-Qed.
-
-Lemma env_add_union1 :
-  forall X e e',
-  env_eq (env_add X (env_union e e')) (env_union (env_add X e) e').
-Proof. intros. symmetry. apply SF.union_add. Qed.
-
-Lemma env_add_union2 :
-  forall X e e',
-  env_eq (env_add X (env_union e e')) (env_union e (env_add X e')).
-Proof.
-  intros. rewrite SF.union_sym. rewrite env_add_union1. rewrite SF.union_sym.
-  apply env_eq_refl.
-Qed.
-
-Lemma env_union_add :
-  forall X X' e e',
-  env_eq (env_union (env_add X e) (env_add X' e')) (env_union e (env_add X (env_add X' e'))).
-Proof.
-  intros. rewrite <- env_add_union1. rewrite env_add_union2. reflexivity.
-Qed.
-
-Lemma env_add_union_singleton2 :
-  forall X e,
-  env_eq (env_add X e) (env_union e (env_singleton X)).
-Proof. auto with set. Qed.
-
-Lemma env_union_neutral :
-  forall e,
-  env_eq (env_union e env_empty) e.
-Proof. auto with set. Qed.
-
-Lemma env_union_assoc :
-  forall e e' e'',
-  env_eq (env_union (env_union e e') e'') (env_union e (env_union e' e'')).
-Proof. auto with set. Qed.
-
-Lemma env_subset_add :
-  forall XS X,
-  env_subset XS (env_add X XS).
-Proof. intros. rewrite env_add_union_singleton2. apply SF.union_subset_1. Qed.
-
-Definition env_subset_union1 :
-  forall e e',
-  env_subset e (env_union e e')
-  := SF.union_subset_1.
-
-Definition env_subset_union2 :
-  forall e e',
-  env_subset e' (env_union e e')
-  := SF.union_subset_2.
-
-Lemma env_union_list_spec :
-  forall xs ys,
-  env_eq (env_union_list xs ys) (env_union xs (list_to_env ys)).
-Proof.
-  unfold SF.of_list. unfold env_union_list. unfold flip. intros. gen xs.
-  induction ys; intros.
-    simpl. rewrite env_union_neutral. reflexivity.
-    simpl in *. rewrite IHys. rewrite <- env_add_union2.
-    rewrite env_add_union1. reflexivity.
-Qed.
-
-Lemma list_to_env_cons :
-  forall x xs,
-  env_eq (list_to_env (x :: xs)) (env_add x (list_to_env xs)).
-Proof. intros. unfold SF.of_list. simpl. reflexivity. Qed.
