src/Msg.v
@@ -4,11 +4,6 @@ Inductive Msg :=
 | mkMsg : nat -> Msg
 .
 
-Definition beq_msg x y :=
-  match (x, y) with
-  | (mkMsg x, mkMsg y) => beq_nat x y
-  end
-.
 
 Lemma eq_Msg_dec :
   forall (M M' : Msg), {M = M'} + {M <> M'}.
