src/Sty.v
@@ -1,6 +1,7 @@
 Require Import Msg Tac Var.
 Require Import TLC.LibLogic.
 
+
 Inductive Sty : Set :=
 | unit : Sty
 | send : Msg -> Sty -> Sty
@@ -11,26 +12,15 @@ Inductive Sty : Set :=
 | var : Var -> Sty
 .
 
+
 Lemma eq_Sty_dec :
   forall (S T : Sty), {S = T} + {S <> T}.
 Proof.
   pose proof eq_Msg_dec. pose proof eq_Var_dec. decide equality; auto.
 Defined.
 
-Fixpoint beq_Sty (S T : Sty) : bool :=
-  match (S, T) with
-  | (unit, unit) => true
-  | (send B S', send B' T') => andb (beq_msg B B') (beq_Sty S' T')
-  | (recv B S', recv B' T') => andb (beq_msg B B') (beq_Sty S' T')
-  | (echoice S1 S2, echoice T1 T2) => andb (beq_Sty S1 T1) (beq_Sty S2 T2)
-  | (ichoice S1 S2, ichoice T1 T2) => andb (beq_Sty S1 T1) (beq_Sty S2 T2)
-  | (mu X S', mu Y T') => andb (beq_var X Y) (beq_Sty S' T')
-  | (var X, var Y) => beq_var X Y
-  | _ => false
-  end
-.
 
-Global Instance Sty_Inhab : Inhab Sty.
+Instance Sty_Inhab : Inhab Sty.
 Proof. constructor. exists unit. trivial. Qed.
 
 
@@ -46,6 +36,7 @@ Inductive StySubSimple : Sty -> Sty -> Prop :=
 | StySubSimple_ichoice2 : forall S1 S2, StySubSimple S2 (ichoice S1 S2)
 .
 Hint Constructors StySubSimple : stysub.
+
 
 Inductive StySub : Sty -> Sty -> Prop :=
 | StySub_StySubSimple : forall S S', StySubSimple S S' -> StySub S S'
