src/Var.v
@@ -1,74 +1,24 @@
 Require Import Tac.
 Require Import Arith Structures.Orders Structures.OrdersFacts.
 
+
 Create HintDb env discriminated.
+
 
 Inductive Var :=
 | mkVar : nat -> Var
 .
 Hint Constructors Var : env.
 
+
 Lemma eq_Var_dec : forall (X Y : Var), {X = Y} + {X <> Y}.
 Proof. decide equality. apply eq_nat_dec. Defined.
 Hint Immediate eq_Var_dec : env.
 
-Definition beq_var x y :=
-  match (x, y) with
-  | (mkVar x', mkVar y') => beq_nat x' y'
-  end
-.
-Hint Unfold beq_var : env.
-
-Lemma beq_var_refl : forall x, true = beq_var x x.
-Proof. intros. destruct x; unfold beq_var; apply beq_nat_refl. Qed.
-Hint Resolve beq_var_refl : env.
-
-Lemma beq_var_true_iff : forall x y, x = y <-> beq_var x y = true.
-Proof with (auto with env).
-  intros. split; intros H.
-    rewrite H; auto with env.
-
-    destruct x; destruct y; unfold beq_var in *. rewrite beq_nat_true_iff in H.
-    rewrite H. auto.
-Qed.
-Hint Resolve beq_var_true_iff : env.
-
-Lemma beq_var_true : forall x y, beq_var x y = true -> x = y.
-Proof with auto. intros. apply beq_var_true_iff... Qed.
-Hint Resolve beq_var_true : env.
-
-Lemma beq_var_false_iff : forall x y, x <> y <-> beq_var x y = false.
-Proof with (auto with env).
-  intros x y. split; intros H; destruct x; destruct y.
-    unfold beq_var. apply beq_nat_false_iff. auto.
-
-    introv contra. rewrite contra in H. rewrite <- beq_var_refl in H.
-    discriminate.
-Qed.
-Hint Resolve beq_var_false_iff : env.
-
-Lemma beq_var_false : forall x y, beq_var x y = false -> x <> y.
-Proof. intros. apply beq_var_false_iff; auto. Qed.
-Hint Resolve beq_var_false : env.
-
-Lemma beq_var_eq : forall x y, x = y -> beq_var x y = true.
-Proof. intros. apply beq_var_true_iff; auto. Qed.
-Hint Resolve beq_var_eq : env.
-
-Lemma beq_var_neq : forall x y, x <> y -> beq_var x y = false.
-Proof. intros. apply beq_var_false_iff; auto. Qed.
-Hint Resolve beq_var_neq : env.
-
-Lemma beq_nat_sym : forall x y, beq_nat x y = beq_nat y x.
-Proof. induction x; intros y; destruct y; simpl; auto. Qed.
-Hint Resolve beq_nat_sym : env.
-
-Lemma beq_var_sym : forall x y, beq_var x y = beq_var y x.
-Proof. intros. destruct x; destruct y; unfold beq_var. apply beq_nat_sym. Qed.
 
 Module VarEq <: DecidableType.
   Definition t := Var.
   Definition eq (x y : Var) := eq x y.
-  Instance eq_equiv : Equivalence eq := @eq_equivalence Var.
+  Instance eq_equiv : Equivalence eq := eq_equivalence.
   Definition eq_dec := eq_Var_dec.
 End VarEq.
